feat: new definitions for memory separation

Arm/Memory/Separate.lean
@@ -1,9 +1,10 @@
 /-
 Copyright (c) 2024 Amazon.com, Inc. or its affiliates. All Rights Reserved.
 Released under Apache 2.0 license as described in the file LICENSE.
-Author(s): Shilpi Goel
+Author(s): Shilpi Goel, Siddharth Bhat
 -/
 import Arm.State
+import Arm.BitVec
 
 section Separate
 
@@ -115,6 +116,504 @@ example : mem_subset (BitVec.ofNat 64 (2^64 - 1)) 0#64 0#64 (BitVec.ofNat 64 (2^
 def mem_legal (a1 a2 : BitVec 64) : Bool :=
   a1 <= a2
 
+/-
+Given two legal memory regions `[a1, a2]` and `[b1, b2]` that are separated,
+it must be the case either:
+  - the first one ends before the second one starts (`a2 < b1`),
+  - or, the first one starts after the second one ends `(a1 > b2)`,
+-/
+theorem lt_or_gt_of_mem_separate_of_mem_legal_of_mem_legal (h : mem_separate a1 a2 b1 b2)
+    (ha : mem_legal a1 a2) (hb : mem_legal b1 b2) :
+    a2 < b1 ∨ a1 > b2 := by
+  unfold mem_separate mem_overlap at h
+  obtain ⟨⟨⟨h₁, h₂⟩, h₃⟩, h₄⟩ := by simpa? using h
+  simp [mem_legal] at ha hb
+  rw [BitVec.le_def] at ha hb
+  rw [BitVec.le_def] at h₁ h₂ h₃ h₄
+  rw [BitVec.lt_def, BitVec.gt_def]
+  by_cases h₅ : a2.toNat < b1.toNat
+  · simp [h₅]
+  · by_cases h₆ : a1.toNat > b2.toNat
+    · simp [h₆]
+    · exfalso
+      rw [BitVec.toNat_sub_eq_toNat_sub_toNat_of_le ha] at h₁ h₂
+      rw [BitVec.toNat_sub_eq_toNat_sub_toNat_of_le hb] at h₃ h₄
+      have h₅' : b1.toNat ≤ a2.toNat := by omega
+      have h₆' : a1.toNat ≤ b2.toNat := by omega
+      rw [BitVec.toNat_sub_eq_toNat_sub_toNat_of_le h₅'] at h₄
+      rw [BitVec.toNat_sub_eq_toNat_sub_toNat_of_le h₆'] at h₂
+      omega
+
+@[simp]
+theorem BitVec.neg_neg (x : BitVec w₁) : - (- x) = x := by
+  apply BitVec.eq_of_toNat_eq
+  simp
+  by_cases h : x.toNat = 0
+  · simp [h]
+  · rw [Nat.mod_eq_of_lt (a := 2^w₁ - x.toNat) (by omega)]
+    rw [Nat.sub_sub_eq_min]
+    rw [Nat.min_def]
+    simp [show ¬ 2^w₁ ≤ x.toNat by omega]
+
+@[simp]
+theorem BitVec.neg_eq_sub_zero (x : BitVec w₁) : - x = 0 - x := by
+  apply BitVec.eq_of_toNat_eq
+  simp
+
+theorem toNat_sub_eq_two_pow_sub_add_of_lt
+    {a b : BitVec w₁} (hab : a.toNat < b.toNat) : (a - b).toNat = 2^w₁ - b.toNat + a.toNat := by
+  simp only [toNat_sub]
+  rw [Nat.mod_eq_of_lt (by omega)]
+
+/--
+Given two legal memory regions `[a1, a2]` and `[b1, b2]`,
+such that either the first one ends before the second one starts (`a2 < b1`),
+or the first one starts after the second one ends `(a1 > b2)`,
+the memory regions are separate.
+-/
+theorem mem_separate_of_lt_or_gt_of_mem_legal_of_mem_legal (h : a2 < b1 ∨ a1 > b2)
+    (ha : mem_legal a1 a2) (hb : mem_legal b1 b2) :
+    mem_separate a1 a2 b1 b2 := by
+  unfold mem_separate mem_overlap
+  simp
+  unfold mem_legal at ha hb
+  simp [mem_legal] at ha hb
+  rw [BitVec.le_def] at ha hb
+  simp only[BitVec.le_def]
+  rw [BitVec.lt_def, BitVec.gt_def] at h
+  rcases h with h | h
+  · rw [toNat_sub_eq_toNat_sub_toNat_of_le ha]
+    have ha1b1 : a1.toNat ≤ b1.toNat := by omega
+    rw [toNat_sub_eq_toNat_sub_toNat_of_le ha1b1]
+    have ha1b2 : a1.toNat ≤ b2.toNat := by omega
+    rw [toNat_sub_eq_toNat_sub_toNat_of_le ha1b2]
+    rw [toNat_sub_eq_toNat_sub_toNat_of_le hb]
+    have ha1b1' : a1.toNat < b1.toNat := by omega
+    rw [toNat_sub_eq_two_pow_sub_add_of_lt ha1b1']
+    rw [toNat_sub_eq_two_pow_sub_add_of_lt h]
+    omega
+  · rw [toNat_sub_eq_toNat_sub_toNat_of_le ha]
+    rw [toNat_sub_eq_toNat_sub_toNat_of_le hb]
+    have ha2b1 : b1.toNat ≤ a2.toNat := by omega
+    rw [toNat_sub_eq_toNat_sub_toNat_of_le ha2b1]
+    have ha1b1 : b1.toNat ≤ a1.toNat := by omega
+    rw [toNat_sub_eq_toNat_sub_toNat_of_le ha1b1]
+    have hb1a1 : b1.toNat < a1.toNat := by omega
+    rw [toNat_sub_eq_two_pow_sub_add_of_lt hb1a1]
+    have hb2a1 : b2.toNat < a1.toNat := by omega
+    rw [toNat_sub_eq_two_pow_sub_add_of_lt hb2a1]
+    omega
+
+/--
+If we express a memory region as `[a..(a+n)]` for `(n : Nat)`,
+and this memory region is legal, then we could not have had any wraparound.
+Thus, it must be the case that (a + n).toNat = a.toNat + n
+-/
+theorem add_lt_of_mem_legal_of_lt
+    (h : mem_legal a (a + n)) :
+    a.toNat + n.toNat < 2^64 := by
+  simp [mem_legal] at h
+  simp [BitVec.le_def, BitVec.toNat_add] at h
+  by_cases hadd : a.toNat + n.toNat < 2^64
+  · assumption
+  · exfalso
+    have ha : a.toNat < 2^64 := a.isLt;
+    have h₂ : a.toNat + n.toNat - 2^64 < 2^64 := by omega
+    have hmod : (a.toNat + n.toNat) % 18446744073709551616 = a.toNat + n.toNat - 2^64 := by
+      rw [Nat.mod_eq_sub_mod]
+      rw [Nat.mod_eq_of_lt h₂]
+      omega
+    rw [hmod] at h
+    omega
+
+/--
+If we express a memory region as `[a..(a+n)]` for `(n : Nat)`,
+and this memory region is legal, then we could not have had any wraparound.
+Thus, it must be the case that (a + n).toNat = a.toNat + n
+-/
+theorem toNat_add_distrib_of_mem_legal_of_lt
+    (h : mem_legal a (a + n)) :
+    (a + n).toNat = a.toNat + n.toNat := by
+  simp [BitVec.add_def]
+  rw [Nat.mod_eq_of_lt]
+  apply add_lt_of_mem_legal_of_lt h
+
 end Separate
+
+
+/-#
+
+### New Memory Model
+
+The new memory model is different from the old one in two ways:
+
+1. It uses (base pointer, length) to keep track of memory regions instead of closed inntervals of [pointer 1, pointer 2].
+2. To faciliatate the new representation, it bakes in the assumption that the memory region is legal
+   (i.e. no wraparound).
+3. More softly, it tries to keep reasoning in terms of `Nat` rather than `BitVec` in order to allow easier
+   automation via `omega` for proving disjointedness / subset assumptions.
+
+All of the new definitions are named after the old definitions with a prime (') after their name.
+For robustness (and confidence), we plan to prove theorems that establish the equivalence of the old and new memory models.
+-/
+section NewDefitions
+
+/--
+`mem_legal' a n` witnessses that `(a + n)` does not overflow, and thus `[a..a+n)` is a valid range
+of memory. Note that the interval is left closed, right open, and thus `n` is the number of bytes in the memory range.
+-/
+def mem_legal' (a : BitVec 64) (n : Nat) : Prop :=
+  a.toNat + n ≤ 2^64
+
+/--
+@bollu: have proof automation exploit this.
+Equation lemma for `mem_legal'`.
+-/
+theorem mem_legal'_def (h : mem_legal' a n) : a.toNat + n ≤ 2^64 := h
+
+/--
+The maximum size of the range we can choose to allocate is 2^64.
+@bollu: have proof automation exploit this.
+-/
+theorem mem_legal'.size_le_two_pow (h : mem_legal' a n) : n ≤ 2 ^ 64 := by
+  rw [mem_legal'] at h
+  omega
+
+/--
+Legal in the new sense implies legal in the old sense.
+-/
+theorem mem_legal_of_mem_legal' (h : mem_legal' a n) :
+    mem_legal a (a + (BitVec.ofNat 64 (n - 1))) := by
+  simp only [mem_legal', mem_legal, BitVec.le_def] at h ⊢
+  rw [BitVec.toNat_add_eq_toNat_add_toNat]
+  simp
+  rw [BitVec.toNat_ofNat]
+  rw [Nat.mod_eq_of_lt (by omega)]
+  omega
+
+
+/--
+Legal in the new sense implies legal in the old sense.
+Note that the subtraction could also have been written as `(b - a).toNat + 1`
+-/
+theorem mem_legal'_of_mem_legal (h: mem_legal a b) : mem_legal' a (b.toNat - a.toNat + 1) := by
+  simp [mem_legal] at h
+  rw [mem_legal']
+  rw [BitVec.le_def] at h
+  omega
+
+def mem_legal'.of_mem_legal'_of_lt (h : mem_legal' a n) (m : Nat) (hm : m ≤ n) :
+    mem_legal' a m := by
+  simp [mem_legal'] at h ⊢
+  omega
+
+/--
+`mem_separate' a an b bn` asserts that two memory regions [a..an) and [b..bn) are separate.
+Note that we use *half open* intervals.
+See also: Why numbering should start at zero (https://www.cs.utexas.edu/~EWD/ewd08xx/EWD831.PDF)
+-/
+structure mem_separate' (a : BitVec 64) (an : Nat) (b : BitVec 64) (bn : Nat) : Prop where
+  ha : mem_legal' a an
+  hb : mem_legal' b bn
+  h : a.toNat + an ≤ b.toNat ∨ a.toNat ≥ b.toNat + bn
+
+-- @[simp]
+theorem BitVec.not_le_eq_lt {a b : BitVec w₁} : (¬ (a ≤ b)) ↔ b < a := by
+  rw [BitVec.le_def, BitVec.lt_def]
+  omega
+
+/-#
+This is a theorem we ought to prove, which establishes the equivalence
+between the old and new defintions of 'mem_separate'.
+However, the proof is finicky, and so we leave it commented for now.
+-/
+/-
+theorem mem_separate_of_mem_separate' (h : mem_separate' a an b bn)
+    (ha' : a' = a + (BitVec.ofNat w₁ (an - 1) ) (hb' : b' = b + (BitVec.ofNat w₁ (bn - 1)))
+    (hlegala : mem_legal a an) (hlegalb: mem_legal b bn) :
+    mem_separate a a' b b' := by
+  simp [mem_separate]
+  simp [mem_overlap]
+  obtain ⟨ha, hb, hsep⟩ := h
+  simp [mem_legal'] at ha hb
+  subst ha'
+  subst hb'
+  apply Classical.byContradiction
+  intro hcontra
+  · sorry
+  · sorry
+-/
+
+/-- `mem_subset' a an b bn` witnesses that `[a..a+an)` is a subset of `[b..b+bn)`-/
+structure mem_subset' (a : BitVec 64) (an : Nat) (b : BitVec 64) (bn : Nat) : Prop where
+  ha : mem_legal' a an
+  hb : mem_legal' b bn
+  hstart : b ≤ a
+  hend : a.toNat + an ≤ b.toNat + bn
+
+theorem mem_subset'_refl (h : mem_legal' a an) : mem_subset' a an a an where
+  ha := h
+  hb := h
+  hstart := by simp [BitVec.le_def]
+  hend := by simp [BitVec.le_def]
+
+/--
+If `[a'..a'+an')` begins at least where `[a..an)` begins,
+and ends before `[a..an)` ends, and if `[a..an)` is a subset of `[b..bn)`,
+then `[a'..a'+an')` is a subset of `[b..bn)`.
+-/
+theorem mem_subset'_of_le_of_le {a' : BitVec 64} (h : mem_subset' a an b bn)
+  (ha' : a.toNat ≤ a'.toNat) (han' : a'.toNat + an' ≤ a.toNat + an) :
+  mem_subset' a' an' b bn where
+  ha := by
+    obtain ⟨ha, hb, hstart, hend⟩ := h
+    simp only [mem_legal', Nat.reducePow] at ha hb ⊢
+    simp_all only [BitVec.le_def]
+    omega
+  hb := h.hb
+  hstart := by
+    obtain ⟨ha, hb, hstart, hend⟩ := h
+    simp only [mem_legal', Nat.reducePow] at ha hb
+    simp_all only [BitVec.le_def]
+    omega
+  hend := by
+    obtain ⟨ha, hb, hstart, hend⟩ := h
+    simp only [mem_legal', Nat.reducePow] at ha hb
+    simp_all only [BitVec.le_def]
+    omega
+
+/--
+If `[a..an)` is a subset of `[b..bn)`,
+then `[a..an')` is a subset of `[b..bn)` if `an' ≤ an`.
+-/
+theorem mem_subset'_of_length_le (h : mem_subset' a an b bn)
+  (han' : an' ≤ an) : mem_subset' a an' b bn := by
+  apply mem_subset'_of_le_of_le h
+  · simp [BitVec.le_def]
+  · omega
+
+/-- if `[a..an) ≤ [b..bn)` and `[b..bn) ⟂ [c..cn)`, then `[a..an) ⟂ [c..cn)`. -/
+theorem mem_separate'_of_mem_separate'_of_mem_subset'
+    (hsep : mem_separate' b bn c cn)
+    (hsub : mem_subset' a an b bn) :
+    mem_separate' a an c cn := by
+  obtain ⟨_, hsep₂, hsep₃⟩ := hsep
+  obtain ⟨hsub₁, _, hsub₃, hsub₄⟩ := hsub
+  simp_all only [BitVec.le_def]
+  constructor <;>
+    solve
+    | omega
+    | assumption
+
+-- theorem Nat.sub_mod_eq (x y : Nat) : (x - y) % t =
+
+private theorem Nat.sub_mod_eq_of_lt_of_le {x y : Nat} (hx : x < n) (hy : y ≤ x) :
+    (x - y) % n = (x % n) - (y % n) := by
+  rw [Nat.mod_eq_of_lt (by omega)]
+  rw [Nat.mod_eq_of_lt (by omega)]
+  rw [Nat.mod_eq_of_lt (by omega)]
+
+theorem BitVec.le_add_self_of_lt (a b : BitVec w₁) (hab : a.toNat + b.toNat < 2^w₁) :
+   a ≤ a + b := by
+  rw [BitVec.le_def]
+  rw [BitVec.toNat_add_eq_toNat_add_toNat (by omega)]
+  omega
+
+theorem BitVec.add_sub_cancel_left {a b : BitVec w₁}
+    (hab : a.toNat + b.toNat < 2^w₁) : (a + b) - a = b := by
+  apply BitVec.eq_of_toNat_eq
+  rw [BitVec.toNat_sub_eq_toNat_sub_toNat_of_le]
+  · rw [BitVec.toNat_add_eq_toNat_add_toNat (by omega)]
+    omega
+  · apply BitVec.le_add_self_of_lt
+    omega
+
+theorem BitVec.le_add_iff_sub_le {a b c : BitVec w₁}
+   (hac : c ≤ a) (hbc : b.toNat + c.toNat < 2^w₁) :
+    (a ≤ b + c) ↔ (a - c ≤ b) := by
+  simp_all only [BitVec.le_def]
+  rw [BitVec.toNat_sub_eq_toNat_sub_toNat_of_le (by rw [BitVec.le_def]; omega)]
+  rw [BitVec.toNat_add_eq_toNat_add_toNat (by omega)]
+  omega
+
+theorem BitVec.sub_le_sub_iff_right (a b c : BitVec w₁) (hac : c ≤ a)
+    (hbc : c ≤ b) : (a - c ≤ b - c) ↔ a ≤ b := by
+  simp_all only [BitVec.le_def]
+  rw [BitVec.toNat_sub_eq_toNat_sub_toNat_of_le (by rw [BitVec.le_def]; omega)]
+  rw [BitVec.toNat_sub_eq_toNat_sub_toNat_of_le (by rw [BitVec.le_def]; omega)]
+  omega
+
+-- mem_subset' is a safe over-approximation of mem_subset.
+theorem mem_subset_of_mem_subset' (h : mem_subset' a an b bn) (han : an > 0) (hbn : bn > 0) :
+  mem_subset a (a + BitVec.ofNat 64 (an - 1)) b (b + BitVec.ofNat 64 (bn - 1)):= by
+  unfold mem_subset
+  obtain ⟨ha, hb, hstart, hend⟩ := h
+  unfold mem_legal' at ha hb
+  simp only [Nat.reducePow, Nat.add_one_sub_one, Bool.or_eq_true, decide_eq_true_eq,
+    Bool.and_eq_true]
+  by_cases hb : bn = 2^64
+  · left
+    apply BitVec.eq_of_toNat_eq
+    rw [BitVec.toNat_sub_eq_toNat_sub_toNat_of_le ]
+    · rw [BitVec.toNat_add_eq_toNat_add_toNat]
+      · simp only [BitVec.toNat_ofNat, Nat.reducePow, Nat.reduceMod]
+        rw [Nat.mod_eq_of_lt (by omega)]
+        omega
+      · simp only [BitVec.toNat_ofNat, Nat.reducePow]
+        rw [Nat.mod_eq_of_lt (by omega)]
+        omega
+    · simp only [BitVec.le_def, BitVec.toNat_add, BitVec.toNat_ofNat, Nat.reducePow,
+      Nat.add_mod_mod]
+      rw [Nat.mod_eq_of_lt (by omega)]
+      omega
+  · have hbn : (BitVec.ofNat 64 (bn - 1)).toNat = (bn - 1) := by simp; omega
+    have han : (BitVec.ofNat 64 (an - 1)).toNat = (an - 1) := by simp; omega
+    rw [BitVec.le_def] at hstart
+    right
+    constructor
+    · rw [BitVec.add_sub_cancel_left]
+      · apply (BitVec.le_add_iff_sub_le _ _).mp
+        · rw [BitVec.le_def, BitVec.toNat_add, han, BitVec.toNat_add, hbn]; omega
+        . rw [BitVec.le_def, BitVec.toNat_add, han]; omega
+        · rw [hbn]; omega
+      · rw [hbn]; omega
+    · rw [BitVec.sub_le_sub_iff_right]
+      · rw [BitVec.le_def, BitVec.toNat_add, han]
+        omega
+      · assumption
+      · rw [BitVec.le_def, BitVec.toNat_add, han]
+        omega
+
+/- value of read_mem_bytes when separate. -/
+theorem read_mem_bytes_write_mem_bytes_eq_read_mem_bytes_of_mem_separate'
+  (hsep : mem_separate' x xn y yn) -- separation
+  (val : BitVec (yn * 8)) :
+    read_mem_bytes xn x (write_mem_bytes yn y val mem) =
+    read_mem_bytes xn x mem := by
+  simp only [Nat.reduceMul, memory_rules,
+    Nat.reduceAdd, BitVec.ofNat_eq_ofNat,
+    BitVec.cast_eq]
+  apply BitVec.eq_of_getLsb_eq
+  intros i
+  obtain ⟨hsrc, hdest, hsplit⟩ := hsep
+  rw [Memory.getLsb_read_bytes, Memory.getLsb_write_bytes, Memory.getLsb_read_bytes]
+  simp only [i.isLt]
+  simp only [decide_True, ite_eq_left_iff, Bool.true_and]
+  intros h₁
+  intros h₂
+  -- we need to make use of mem_separate to show that src_addr + i / 8 < dest_addr | src_addr + i/7 ≥ dest_addr + 16
+  exfalso
+  · rcases hsplit with this | this
+    · simp [BitVec.le_def] at h₁
+      omega
+    · have hcontra_h2 : x.toNat + 16 < y.toNat + 16 := by
+        simp at this
+        have hi : (i : Nat) / 8 < xn := by
+          apply Nat.div_lt_of_lt_mul
+          simp [Nat.mul_comm]
+        rw [BitVec.toNat_add_eq_toNat_add_toNat] at h₂
+        · omega
+        · have := mem_legal'_def hsrc
+          apply Nat.lt_of_lt_of_le _ this
+          apply Nat.add_lt_add_iff_left.mpr
+          simp
+          rw [Nat.mod_eq_of_lt]
+          omega
+          omega
+      omega
+  · have := hsrc.size_le_two_pow
+    omega
+  · have := mem_legal'_def hdest
+    omega
+  · have := hsrc.size_le_two_pow
+    omega
+
+theorem BitVec.toNat_ofNat_lt {n w₁ : Nat} (hn : n < 2^w₁) :
+    (BitVec.ofNat w₁ n).toNat = n := by
+  simp only [toNat_ofNat, Nat.mod_eq_of_lt hn]
+
+theorem BitVec.ge_of_not_lt (x y : BitVec w₁) (h : ¬ (x < y)) : x ≥ y := by
+  simp_all only [BitVec.le_def, BitVec.lt_def]
+  omega
+
+/- value of `read_mem_bytes'` when subset. -/
+theorem read_mem_bytes_write_mem_bytes_eq_extract_LsB_of_mem_subset
+  (hsep : mem_subset' x xn y yn) -- subset relation.
+  (val : BitVec (yn * 8)) :
+    Memory.read_bytes xn x (Memory.write_bytes yn y val mem) =
+      val.extractLsBytes (x.toNat - y.toNat) xn := by
+  apply BitVec.eq_of_getLsb_eq
+  intros i
+  obtain ⟨hx, hy, hstart, hend⟩ := hsep
+
+  obtain hx' := hx.size_le_two_pow
+  obtain hy' := mem_legal'_def hy
+
+  rw [Memory.getLsb_read_bytes (by omega)]
+  rw [Memory.getLsb_write_bytes (by omega)]
+  rw [BitVec.getLsb_extractLsByte]
+  rw [BitVec.getLsb_extractLsBytes]
+  by_cases hxn : xn = 0
+  · subst hxn
+    exfalso
+    have h := i.isLt
+    simp at h
+  · simp only [show (0 < xn) by omega]
+    simp only [show ((x.toNat - y.toNat) * 8 + xn * 8 - 1 - (x.toNat - y.toNat) * 8) = xn * 8 - 1 by omega]
+    by_cases h₁ : ↑i < xn * 8
+    · simp only [h₁]
+      simp only [show (i ≤ xn * 8 - 1) by omega]
+      simp only [decide_True, Bool.true_and]
+      obtain ⟨i, hi⟩ := i
+      simp only at h₁
+      simp only []
+      have h₁' : (BitVec.ofNat 64 (i / 8)).toNat = (i / 8) := by
+        apply BitVec.toNat_ofNat_lt
+        omega
+      have hadd : (x + BitVec.ofNat 64 (↑i / 8)).toNat = x.toNat + (i / 8) := by
+        rw [BitVec.toNat_add_eq_toNat_add_toNat (by omega)]
+        rw [BitVec.toNat_ofNat_lt (by omega)]
+      simp only [BitVec.lt_def]
+      simp only [hadd]
+      by_cases h₂ : (x.toNat + i/ 8) < y.toNat
+      · -- contradiction
+        exfalso
+        rw [BitVec.le_def] at hstart
+        omega
+      · simp only [h₂, if_false]
+        by_cases h₃ : x.toNat + i / 8 ≥ y.toNat + yn
+        · rw [BitVec.le_def] at hstart
+          omega
+        · simp only [h₃, if_false]
+          simp only [show i % 8 ≤ 7 by omega]
+          simp only [decide_True, Bool.true_and]
+          -- ⊢ val.getLsb ((x + BitVec.ofNat 64 (i / 8) - y).toNat * 8 + i % 8) = val.getLsb ((y.toNat - x.toNat) * 8 + i)
+          /-
+          This is clearly true, it simplifes to (x.toNat - y.toNat) * 8 + (i/8)*8 + i % 8.
+          which equals (x.toNat - y.toNat + i)
+          -/
+          congr 1
+          rw [BitVec.toNat_sub_eq_toNat_sub_toNat_of_le (by rw [BitVec.le_def]; omega)]
+          rw [BitVec.toNat_add_eq_toNat_add_toNat (by omega)]
+          rw [BitVec.toNat_ofNat_lt (by omega)]
+          have himod : (i / 8) * 8 + (i % 8) = i := by omega
+          rw [Nat.mul_sub_right_distrib, Nat.mul_sub_right_distrib,
+            Nat.add_mul]
+          conv =>
+            rhs
+            rw [← himod]
+          rw [BitVec.le_def] at hstart
+          omega
+    · simp [h₁]
+      intros h
+      apply BitVec.getLsb_ge
+      omega
+
+/--
+info: 'read_mem_bytes_write_mem_bytes_eq_extract_LsB_of_mem_subset' depends on axioms: [propext, Classical.choice, Quot.sound]
+-/
+#guard_msgs in #print axioms read_mem_bytes_write_mem_bytes_eq_extract_LsB_of_mem_subset
+
+
 
 ----------------------------------------------------------------------
